test.fst
@@ -1,0 +1,58 @@
+module Set
+(* This example uses (list 'a) to model a set of 'a-typed elements. *)
+type set :: * => * = list
+
+(* Axiomatizing set membership using the predicate In *)
+type In :: 'a::* => 'a => list 'a => E
+assume In_hd: forall (hd:'a) (tl:list 'a). (In hd (Cons hd tl))
+assume In_tl: forall (hd:'a) (x:'a) (tl:list 'a). (In x tl) => (In x (Cons hd tl))
+assume notinNil: forall (x:'a). not (In x Nil)
+assume notinCons: forall (x:'a) (y:'a) (tl:list 'a). ((not (In x tl)) && (not (x=y))) => not (In x (Cons y tl))
+
+(*   
+   A function to decide set membership 
+*)
+val member: x:'a -> s:set 'a -> (b:bool{b=true <=> In x s})
+let rec member x = function
+  | [] -> false
+  | hd::tl -> if hd=x then true else member x tl
+
+(*
+   We can define set union as list append, and give it a specification that
+   (union x y) contains all the elements from x and y, and nothing else.
+*)
+val union: x:set 'a -> y:set 'a -> z:set 'a{forall a. In a z <=> (In a x || In a y)}
+let rec union x y = match x with
+  | [] -> y
+  | a::tl -> a::(union tl y)
+
+(*
+   It's often convenient to use abbreviations for big refined types:
+   (isect x y) is the type of a set that's the intersection of x and y
+*)
+type isect 'a (x:set 'a) (y:set 'a) = z:set 'a{forall a. In a z <=> (In a x && In a y)}
+val intersect: x:set 'a -> y:set 'a -> isect x y
+let rec intersect x y = match x with
+  | [] -> []
+  | hd::tl ->
+      if member hd y
+      then hd::(intersect tl y)
+      else intersect tl y
+
+(* A tail recursive version of intersect *)
+type isectplus 'a (x:set 'a) (y:set 'a) (o:set 'a) =
+    z:set 'a{forall a. In a z <=> ((In a o) || (In a x && In a y))}
+
+val aux: out:set 'a -> x:set 'a -> y:set 'a -> isectplus x y out
+let rec aux out x y =
+  match x with
+    | [] -> out
+    | hd::tl ->
+        if member hd y
+        then aux (hd::out) tl y
+        else aux out tl y
+
+val intersect' : x:set 'a -> y:set 'a -> isect x y
+let intersect' x y = aux [] x y
+
+end
