Makefile
@@ -14,5 +14,9 @@ crypto:
 	mkdir -p bin
 	fstar --genIL --writePrims --odir bin --dotnet4 --parallel simplecrypto.fst
 
+test:
+	mkdir -p bin
+	fstar --genIL --writePrims --odir bin --dotnet4 --parallel test.fst	
+
 clean:
 	rm -rf bin
