build.ps1
@@ -1,0 +1,2 @@
+mkdir -p bin
+fstar --genIL --writePrims --odir bin --dotnet4 --parallel simplesaml.fst
